src/3d/prelude/EverParse3d.Actions.Base.fst
@@ -1953,7 +1953,7 @@ let probe_then_validate
       (v:validate_with_action_t p inv disj l ha allow_reading)
       (src:U64.t)
       (dest:CP.copy_buffer_t)
-      (probe:CP.probe_m)
+      (probe:CP.probe_m unit)
   = fun ctxt error_handler_fn input input_length pos posf ->
       CP.properties dest;
       let h0 = HST.get () in
